src/SepLogic.v
@@ -1,3 +1,0 @@
-Require Export
-        SepLogic.Mem
-        SepLogic.Pred.
